finished mscIsMaximum along with a few other lemmas

Pearls/SurpassingElements.dfy
@@ -89,6 +89,49 @@ module SurpassingProblem {
     FoldRight(maxNat, xs, xs[0])
   }
 
+  lemma LemmaMaximumOne(xs: seq<nat>)
+    requires |xs| == 1
+    ensures maximum(xs) == xs[0]
+  {
+    calc{
+      maximum(xs);
+      FoldRight(maxNat, xs, xs[0]);
+      maxNat(xs[0], FoldRight(maxNat, xs[1..], xs[0]));
+      maxNat(xs[0], FoldRight(maxNat, [], xs[0]));
+      maxNat(xs[0], xs[0]);
+      xs[0];
+    }
+  }
+
+    lemma LemmaFoldRightMaxOrInit(xs: seq<nat>, init: nat)
+    ensures FoldRight(maxNat, xs, init) == init || FoldRight(maxNat, xs, init) in xs
+  {
+    if |xs| == 0 {
+    } else {
+      LemmaFoldRightMaxOrInit(xs[1..], init);
+      
+    }
+  }
+
+   lemma LemmaMaximumIn(xs: seq<nat>)
+    requires |xs| > 0
+    ensures maximum(xs) in xs
+  {
+    if |xs| == 1 {
+      calc {
+        maximum(xs);
+        FoldRight(maxNat, xs, xs[0]);
+        maxNat(xs[0], FoldRight(maxNat, [], xs[0]));
+        maxNat(xs[0], xs[0]);
+        xs[0];
+      }
+      assert maximum(xs) in xs;
+    } else {
+      assert maximum(xs) == FoldRight(maxNat, xs, xs[0]);
+      LemmaFoldRightMaxOrInit(xs, xs[0]);
+    }
+  }
+
   lemma LemmaFoldRightMax(xs: seq<nat>, init: nat)
     ensures forall x :: x in xs ||x in {init} ==> FoldRight(maxNat, xs, init) >= x
   {
@@ -112,72 +155,121 @@ module SurpassingProblem {
       LemmaFoldRightMax(xs, xs[0]);
     }
   }
+
+ lemma LemmaFoldRightMaxAssoc(xs: seq<nat>, init: nat)
+    requires |xs| > 0
+    ensures FoldRight(maxNat, xs, init) == maxNat(maximum(xs), init)
+  {
+    if |xs| == 1 {
+      // Base case: [x]. FoldRight result is max(x, init). maximum is x.
+
+      calc {
+        maximum(xs);
+        // Definition
+        FoldRight(maxNat, xs, xs[0]);
+        // Unroll recursive step: f(head, FoldRight(tail, init))
+        maxNat(xs[0], FoldRight(maxNat, [], xs[0]));
+        // Unroll base case: FoldRight([], init) == init
+        maxNat(xs[0], xs[0]);
+        // Property of Max
+        xs[0];
+      }
+
+    } else {
+      // Inductive step: xs = [x] + tail
+      // 1. Unroll FoldRight definition
+      assert FoldRight(maxNat, xs, init) == maxNat(xs[0], FoldRight(maxNat, xs[1..], init));
+      
+      // 2. Apply IH to tail
+      LemmaFoldRightMaxAssoc(xs[1..], init);
+      // Now we have: maxNat(xs[0], maxNat(maximum(xs[1..]), init))
+      
+      // 3. Apply IH to definition of maximum(xs) to simplify it
+      // maximum(xs) == FoldRight(..., xs[0])
+      LemmaFoldRightMaxAssoc(xs[1..], xs[0]);
+      // maximum(xs) == maxNat(xs[0], maximum(xs[1..]))
+      
+      // 4. Associativity/Commutativity logic (automatically handled by Dafny for maxNat)
+      // max(a, max(b, c)) == max(max(a, b), c)
+    }
+  }
+
   lemma LemmaMaximumConcat(xs: seq<nat>, ys: seq<nat>)
     requires |ys| > 0
     requires |xs| > 0
     ensures maximum(xs+ys) == maxNat(maximum(xs), maximum(ys))
   {
-    if |xs| == 1 {
-
-    }else{
-      LemmaMaximumConcat(xs[1..], ys);
+    calc {
+      maximum(xs + ys);
+      // 1. Expand definition
+      FoldRight(maxNat, xs + ys, (xs + ys)[0]);
+      { assert (xs + ys)[0] == xs[0]; }
+      FoldRight(maxNat, xs + ys, xs[0]);
+      
+      // 2. Distribute over concat (using your previous lemma)
+      { LemmaFoldRightDistributesOverConcat(maxNat, xs[0], xs, ys); }
+      FoldRight(maxNat, xs, FoldRight(maxNat, ys, xs[0]));
+      
+      // 3. Use Helper on the inner part (ys) to decouple xs[0]
+      { LemmaFoldRightMaxAssoc(ys, xs[0]); }
+      FoldRight(maxNat, xs, maxNat(maximum(ys), xs[0]));
+      
+      // 4. Use Helper on the outer part (xs)
+      { LemmaFoldRightMaxAssoc(xs, maxNat(maximum(ys), xs[0])); }
+      maxNat(maximum(xs), maxNat(maximum(ys), xs[0]));
+      
+      // 5. Associativity and Simplification
+      // max(A, max(B, C)) == max(max(A, C), B)
+      maxNat(maxNat(maximum(xs), xs[0]), maximum(ys));
+      
+      // 6. Observe that max(maximum(xs), xs[0]) is just maximum(xs)
+      // (Because xs[0] is already contained in maximum(xs))
+      { 
+         LemmaFoldRightMaxAssoc(xs, xs[0]); 
+         // This implies maximum(xs) == maxNat(maximum(xs), xs[0])
+      }
+      maxNat(maximum(xs), maximum(ys));
     }
   }
 
-  lemma LemmaMaximumIn(xs: seq<nat>)
-    requires |xs| > 0
-    ensures maximum(xs) in xs
-  {
-    if |xs| == 1 {
-      calc {
-        maximum(xs);
-        FoldRight(maxNat, xs, xs[0]);
-        maxNat(xs[0], FoldRight(maxNat, xs[1..], xs[0]));
-        maxNat(xs[0], FoldRight(maxNat, [], xs[0]));
-        maxNat(xs[0], xs[0]);
-        xs[0];
-      }
-      assert maximum(xs) in xs;
-    }else{
-      assert xs == [xs[0]]+xs[1..];
-      LemmaMaximumIn(xs[1..]);
-      LemmaFoldRightDistributesOverConcat(maxNat,xs[0], [xs[0]],xs[1..]);
-
-      calc {
-        maximum(xs);
-        FoldRight(maxNat, xs, xs[0]);
-        FoldRight(maxNat, [xs[0]], FoldRight(maxNat, xs[1..], xs[0]));
-        // maxNat(xs[0], FoldRight(maxNat, xs[1..], xs[0]));
-      }
-      if xs[0] >  maximum(xs[1..]) {
-
-        assert maximum(xs) in xs;
-      }else{
-
-        assert maximum(xs) in xs;
-      }
-      assert maximum(xs) in xs;
-
-    }
+  predicate lt(a: int, b: int) {
+    a < b
   }
+
 
   ghost function maxScount(xs: seq<int>): nat
     requires |xs| > 0
   {
     ThereIsAMaxScount(xs);
-    var m :| 0 <= m < |xs| && forall i :: 0 <= i < |xs| ==> scount(xs[m..][0], xs[m..][1..], (a,b) => a <b) >= scount(xs[i..][0], xs[i..][1..], (a,b) => a <b);
-    scount(xs[m..][0], xs[m..][1..], (a,b) => a < b)
+    var m :| 0 <= m < |xs| && forall i :: 0 <= i < |xs| ==> scount(xs[m..][0], xs[m..][1..], lt) >= scount(xs[i..][0], xs[i..][1..], lt);
+    scount(xs[m..][0], xs[m..][1..], lt)
   }
+
+  lemma LemmaMaxScountEquivalence(xs: seq<int>, m: nat, n: nat)
+    requires 0 <= m < |xs| && forall i :: 0 <= i < |xs| ==> scount(xs[m..][0], xs[m..][1..], lt) >= scount(xs[i..][0], xs[i..][1..], lt)
+    requires 0 <= n < |xs| && forall i :: 0 <= i < |xs| ==> scount(xs[n..][0], xs[n..][1..], lt) >= scount(xs[i..][0], xs[i..][1..], lt)
+    ensures scount(xs[m..][0], xs[m..][1..], lt) == scount(xs[n..][0], xs[n..][1..], lt)
+  {
+
+  }
+
+  function mscMapper(zs: seq<int>): nat
+    // requires |zs| > 0
+  {
+    assume |zs| > 0;
+    scount(zs[0], zs[1..], lt)
+  } 
 
   function msc(xs: seq<int>): nat
     requires |xs| > 0
   {
-    var zzs := Map((zs) => assume |zs| > 0;
-                     scount(zs[0], zs[1..], (a,b)=> a < b), Tails(xs));
+    var zzs := Map(mscMapper, Tails(xs));
     maximum(zzs)
   }
 
-  lemma {:isolate_assertions} mscIsMaximum(xs: seq<int>)
+  function Score(xs: seq<int>): nat requires |xs| > 0 { scount(xs[0], xs[1..], (a,b) => a < b) }
+
+  lemma mscIsMaximum(xs: seq<int>)
     requires |xs| > 0
     ensures msc(xs) == maxScount(xs)
   {
@@ -186,37 +278,108 @@ module SurpassingProblem {
       assert Tails(xs) == [xs] + Tails(xs[1..]);
       assert Tails(xs) == [xs];
       assert Filter(xxs => |xxs| > 0, Tails(xs)) == [xs];
-      assert scount(xs[0..][0], xs[0..][1..], (a,b) => a <b) == scount(xs[0], xs[1..], (a,b) => a <b);
+      assert scount(xs[0..][0], xs[0..][1..], lt) == scount(xs[0], xs[1..], lt);
       ThereIsAMaxScount(xs);
-      var m :| 0 <= m < |xs| && forall i :: 0 <= i < |xs| ==> scount(xs[m..][0], xs[m..][1..], (a,b) => a <b) >= scount(xs[i..][0], xs[i..][1..], (a,b) => a <b);
+      var m :| 0 <= m < |xs| && forall i :: 0 <= i < |xs| ==> scount(xs[m..][0], xs[m..][1..], lt) >= scount(xs[i..][0], xs[i..][1..], lt);
       assert m == 0;
+      var zzs := Map(mscMapper, Tails(xs));
+      calc {
+        Map(mscMapper, Tails(xs));
+        Map(mscMapper, [xs]);
+        [mscMapper(xs)]+Map(mscMapper, [xs][1..]);
+        [mscMapper(xs)]+Map(mscMapper, []);
+      }
+      assert zzs == [scount(xs[0], xs[1..], lt)];
+      calc {
+        maximum(zzs);
+        FoldRight(maxNat, zzs, zzs[0]);
+        maxNat(zzs[0], FoldRight(maxNat, zzs[1..], zzs[0]));
+        maxNat(zzs[0], FoldRight(maxNat, [], zzs[0]));
+        maxNat(zzs[0], zzs[0]);
+        zzs[0];
+      }
+      assert msc(xs) == scount(xs[0], xs[1..], lt);
       assert msc(xs) == maxScount(xs);
     }else{
       mscIsMaximum(xs[1..]);
       assert xs == [xs[0]]+xs[1..];
+      assert Tails(xs) == [xs] + Tails(xs[1..]);
+      calc {
+        msc(xs);
+        maximum(Map(mscMapper, Tails(xs)));
+        maximum(Map(mscMapper, [xs] + Tails(xs[1..])));
+        maximum([mscMapper(xs)]+Map(mscMapper,Tails(xs[1..])));
+        {LemmaMaximumConcat([mscMapper(xs)],Map(mscMapper,Tails(xs[1..])));}
+        maxNat(maximum([mscMapper(xs)]),maximum(Map(mscMapper,Tails(xs[1..]))));
+        maxNat(maximum([mscMapper(xs)]),msc(xs[1..]));
+        {LemmaMaximumOne([mscMapper(xs)]);}
+        maxNat(mscMapper(xs),msc(xs[1..]));
+
+      }
+      ThereIsAMaxScount(xs);
+      ThereIsAMaxScount(xs[1..]);
+      LemmaMaximum(Map(mscMapper, Tails(xs)));
+      var m :| 0 <= m < |xs| && forall i :: 0 <= i < |xs| ==> scount(xs[m..][0], xs[m..][1..], lt) >= scount(xs[i..][0], xs[i..][1..], lt);
+      var m' :| 0 <= m' < |xs| && forall i :: 0 <= i < |xs| ==> scount(xs[m'..][0], xs[m'..][1..], lt) >= scount(xs[i..][0], xs[i..][1..], lt) && maxScount(xs) == scount(xs[m'..][0], xs[m'..][1..], lt);
+      LemmaMaxScountEquivalence(xs, m, m');
+      LemmaMaximum(Map(mscMapper, Tails(xs[1..])));
+      var n :| 0 <= n < |xs[1..]| && forall i :: 0 <= i < |xs[1..]| ==> scount(xs[1..][n..][0], xs[1..][n..][1..], lt) >= scount(xs[1..][i..][0], xs[1..][i..][1..], lt) && maxScount(xs[1..]) == scount(xs[1..][n..][0], xs[1..][n..][1..], lt);
+      assert msc(xs[1..]) == maxScount(xs[1..]);
+      assert maxScount(xs[1..]) == scount(xs[1..][n..][0], xs[1..][n..][1..], lt);
+      if mscMapper(xs) > msc(xs[1..]) {
+        assert msc(xs) == mscMapper(xs);
+        assert m == 0 by {
+          if m != 0 {
+            assert scount(xs[m..][0], xs[m..][1..], lt) == scount(xs[1..][m-1..][0], xs[1..][m-1..][1..], lt);
+            assert scount(xs[m..][0], xs[m..][1..], lt) <= scount(xs[1..][n..][0], xs[1..][n..][1..], lt);
+            assert mscMapper(xs) == scount(xs[0..][0], xs[0..][1..], lt);
+            assert mscMapper(xs) > scount(xs[1..][n..][0], xs[1..][n..][1..], lt);
+            assert false;
+          }
+        }
+        assert msc(xs) == maxScount(xs);
+      }else{
+        assert msc(xs) == msc(xs[1..]);
+        assert scount(xs[1..][n..][0], xs[1..][n..][1..], lt) == scount(xs[n+1..][0], xs[n+1..][1..], lt);
+        forall i | 0 <= i < |xs| 
+          ensures scount(xs[n+1..][0], xs[n+1..][1..], lt) >= scount(xs[i..][0], xs[i..][1..], lt)
+        {
+          if i == 0 {
+            assert scount(xs[n+1..][0], xs[n+1..][1..], lt) >= scount(xs[i..][0], xs[i..][1..], lt);
+          }else{
+            assert scount(xs[i..][0], xs[i..][1..], lt) == scount(xs[1..][i-1..][0], xs[1..][i-1..][1..], lt);
+            assert scount(xs[n+1..][0], xs[n+1..][1..], lt) >= scount(xs[i..][0], xs[i..][1..], lt);
+          }
+        }
+        LemmaMaxScountEquivalence(xs, n+1, m');
+        // assert m == n+1;
+        assert msc(xs) == maxScount(xs);
+      }
+      // LemmaMaximumConcat([xs[0]],xs[1..]);
+      // LemmaMaximumOne([xs[0]]);
       assert msc(xs) == maxScount(xs);
     }
   }
 
   lemma ThereIsAMaxScount(xs: seq<int>)
     requires |xs| > 0
-    ensures exists m :: 0 <= m < |xs| && forall i :: 0 <= i < |xs| ==> scount(xs[m..][0], xs[m..][1..], (a,b) => a <b) >= scount(xs[i..][0], xs[i..][1..], (a,b) => a <b)
+    ensures exists m :: 0 <= m < |xs| && forall i :: 0 <= i < |xs| ==> scount(xs[m..][0], xs[m..][1..], lt) >= scount(xs[i..][0], xs[i..][1..], lt)
   {
     if |xs| == 1 {
       assert xs[1..] == [];
-      assert scount(xs[0..][0], xs[0..][1..], (a,b) => a <b) == scount(xs[0], xs[1..], (a,b) => a <b);
-      assert exists m :: 0 <= m < |xs| && forall i :: 0 <= i < |xs| ==> scount(xs[m..][0], xs[m..][1..], (a,b) => a <b) >= scount(xs[i..][0], xs[i..][1..], (a,b) => a <b);
+      assert scount(xs[0..][0], xs[0..][1..], lt) == scount(xs[0], xs[1..], lt);
+      assert exists m :: 0 <= m < |xs| && forall i :: 0 <= i < |xs| ==> scount(xs[m..][0], xs[m..][1..], lt) >= scount(xs[i..][0], xs[i..][1..], lt);
     }else{
       ThereIsAMaxScount(xs[1..]);
-      var m :| 0 <= m < |xs[1..]| && forall i :: 0 <= i < |xs[1..]| ==> scount(xs[1..][m..][0], xs[1..][m..][1..], (a,b) => a <b) >= scount(xs[1..][i..][0], xs[1..][i..][1..], (a,b) => a <b);
+      var m :| 0 <= m < |xs[1..]| && forall i :: 0 <= i < |xs[1..]| ==> scount(xs[1..][m..][0], xs[1..][m..][1..], lt) >= scount(xs[1..][i..][0], xs[1..][i..][1..], lt);
       assert xs == [xs[0]]+xs[1..];
       assert xs[1..][m..] == xs[m+1..];
-      assert scount(xs[0..][0], xs[0..][1..], (a,b) => a <b) == scount(xs[0], xs[1..], (a,b) => a <b);
+      assert scount(xs[0..][0], xs[0..][1..], lt) == scount(xs[0], xs[1..], lt);
       assert forall i :: 0 <= i < |xs[1..]| ==> xs[1..][i..] == xs[i+1..];
-      if scount(xs[0], xs[1..], (a,b) => a <b) > scount(xs[1..][m..][0], xs[1..][m..][1..], (a,b) => a <b) {
+      if scount(xs[0], xs[1..], lt) > scount(xs[1..][m..][0], xs[1..][m..][1..], lt) {
 
         forall i | 0 <= i < |xs|
-          ensures scount(xs[0], xs[1..], (a,b) => a <b) >= scount(xs[i..][0], xs[i..][1..], (a,b) => a <b);
+          ensures scount(xs[0], xs[1..], lt) >= scount(xs[i..][0], xs[i..][1..], lt);
         {
           if i == 0 {
           }else{
@@ -226,18 +389,18 @@ module SurpassingProblem {
         }
       }else{
         forall i | 0 <= i < |xs|
-          ensures scount(xs[m+1..][0], xs[m+1..][1..], (a,b) => a <b) >= scount(xs[i..][0], xs[i..][1..], (a,b) => a <b);
+          ensures scount(xs[m+1..][0], xs[m+1..][1..], lt) >= scount(xs[i..][0], xs[i..][1..], lt);
         {
           if i == 0 {
-            assert scount(xs[m+1..][0], xs[m+1..][1..], (a,b) => a <b) >= scount(xs[0], xs[1..], (a,b) => a <b);
+            assert scount(xs[m+1..][0], xs[m+1..][1..], lt) >= scount(xs[0], xs[1..], lt);
           }else{
             assert xs[i..] == xs[1..][(i-1)..];
-            assert scount(xs[i..][0], xs[i..][1..], (a,b) => a <b) == scount(xs[1..][(i-1)..][0], xs[1..][i-1..][1..], (a,b) => a <b);
-            assert scount(xs[m+1..][0], xs[m+1..][1..], (a,b) => a <b) >= scount(xs[i..][0], xs[i..][1..], (a,b) => a <b);
+            assert scount(xs[i..][0], xs[i..][1..], lt) == scount(xs[1..][(i-1)..][0], xs[1..][i-1..][1..], lt);
+            assert scount(xs[m+1..][0], xs[m+1..][1..], lt) >= scount(xs[i..][0], xs[i..][1..], lt);
           }
         }
       }
-      assert exists m :: 0 <= m < |xs| && forall i :: 0 <= i < |xs| ==> scount(xs[m..][0], xs[m..][1..], (a,b) => a <b) >= scount(xs[i..][0], xs[i..][1..], (a,b) => a <b);
+      assert exists m :: 0 <= m < |xs| && forall i :: 0 <= i < |xs| ==> scount(xs[m..][0], xs[m..][1..], lt) >= scount(xs[i..][0], xs[i..][1..], lt);
 
     }
   }
